FixIsMu/UValFI/UVal.v
@@ -31,29 +31,20 @@ Module I.
   Include StlcIso.CanForm.
 End I.
 
-Fixpoint UValFI (n : nat) (τ : I.Ty) {P : ClosedTy τ} {struct n} : F.Ty :=
+Fixpoint UValFI (n : nat) (τ : I.Ty) {struct n} : F.Ty :=
   match n with
     | 0 => F.tunit
     | S n =>
-      let τl := match τ as τ' return (τ = τ' -> _) with
-      | I.tunit => fun _ => F.tunit
-      | I.tarr τ1 τ2 as τ => fun H =>
-        let P1 := closed_arr_implies_closed_argty_eq P H in
-        let P2 := closed_arr_implies_closed_retty_eq P H in
-        let σ1 := @UValFI n τ1 P1 in
-        let σ2 := @UValFI n τ2 P2 in
-        F.tarr σ1 σ2
-      | I.tsum τ1 τ2 => fun H =>
-        let P1 := closed_sum_implies_closed_lhs_eq P H in
-        let P2 := closed_sum_implies_closed_rhs_eq P H in
-        let σ1 := @UValFI n τ1 P1 in
-        let σ2 := @UValFI n τ2 P2 in
+      let τl := match τ with
+      | I.tunit => F.tunit
+      | I.tarr τ1 τ2 as τ => F.tarr (UValFI n τ1) (UValFI n τ2)
+      | I.tsum τ1 τ2 =>
+        let σ1 := UValFI n τ1 in
+        let σ2 := UValFI n τ2 in
         F.tsum σ1 σ2
-      | I.trec τ => fun H =>
-        let P := closed_rec_implies_closed_unfold_eq P H in
-        @UValFI n τ[beta1 (I.trec τ)] P
-      | I.tvar i => fun H => match closed_implies_not_var_eq P i H with end
-      end eq_refl
+      | I.trec τ => UValFI n τ[beta1 (I.trec τ)]
+      | I.tvar i => F.tunit
+      end
       in F.tsum τl F.tunit
   end.
 
@@ -72,7 +63,7 @@ Proof.
   simpl; trivial.
 Qed.
 
-Lemma unkUValT {Γ n τ} {P : ClosedTy τ} {Q : n > 0} : F.Typing Γ unkUVal (@UValFI n τ P).
+Lemma unkUValT {Γ n τ} {P : ClosedTy τ} {Q : n > 0} : F.Typing Γ unkUVal (UValFI n τ).
 Proof.
   induction n.
   inversion Q.
@@ -183,128 +174,133 @@ Qed.
 (* (t : F.Tm) {P : F.Typing t (UValFI n I.tunit)} : F.Tm := *)
 Definition case_uvalfi_unit (n : nat) : F.Tm :=
   let P := UnitClosed 0 in
-  let τ := @UValFI (S n) I.tunit P in
+  let τ := UValFI (S n) I.tunit in
   let t := F.caseof (F.var 0) (F.var 0) (F.Om F.tunit) in
   F.abs τ t.
 
-Definition case_uvalfi_arr (n : nat) (τ1 τ2 : I.Ty) {P1 : ClosedTy τ1} {P2 : ClosedTy τ2} : F.Tm :=
-  let P := FnClosed 0 P1 P2 in
-  let τ := @UValFI (S n) (I.tarr τ1 τ2) P in
-  let τ' := F.tarr (@UValFI n τ1 P1) (@UValFI n τ2 P2) in
+Definition case_uvalfi_arr (n : nat) (τ1 τ2 : I.Ty) : F.Tm :=
+  let τ := @UValFI (S n) (I.tarr τ1 τ2) in
+  let τ' := F.tarr (UValFI n τ1) (UValFI n τ2) in
   let t := F.caseof (F.var 0) (F.var 0) (F.Om τ') in
   F.abs τ t.
 
-Lemma uvalfi_expand_arr {n τ1 τ2 P1 P2} :
-  @UValFI (S n) (I.tarr τ1 τ2) (FnClosed 0 P1 P2) = F.tsum (F.tarr (@UValFI n τ1 P1) (@UValFI n τ2 P2)) F.tunit.
+Lemma uvalfi_expand_arr {n τ1 τ2} :
+  UValFI (S n) (I.tarr τ1 τ2) = F.tsum (F.tarr (UValFI n τ1) (UValFI n τ2)) F.tunit.
 Proof.
-  simpl.
   reflexivity.
-Admitted.
+Qed.
 
-Lemma case_uval_arr_typing {Γ n τ1 τ2 P1 P2} :
+Lemma case_uval_arr_typing {Γ n τ1 τ2} :
   let τ := I.tarr τ1 τ2 in
-  let P := FnClosed 0 P1 P2 in
-  let uval_dest := @case_uvalfi_arr n τ1 τ2 P1 P2 in
-  let arg_type := @UValFI (S n) τ P in
-  let ret_type := (F.tarr (@UValFI n τ1 P1) (@UValFI n τ2 P2)) in
+  let uval_dest := case_uvalfi_arr n τ1 τ2 in
+  let arg_type := UValFI (S n) τ in
+  let ret_type := F.tarr (UValFI n τ1) (UValFI n τ2) in
   let type := F.tarr arg_type ret_type in
   F.Typing Γ uval_dest type.
 Proof.
   intros.
+  unfold uval_dest.
+  unfold type.
+  unfold arg_type.
+  unfold ret_type.
   (* unfold uval_dest, arg_type, ret_type, type, case_uvalfi_arr. *)
   (* crushTyping. *)
   constructor.
+  unfold τ.
   apply (@F.WtCaseof (F.evar Γ arg_type) (F.var 0) (F.var 0) (F.Om ret_type) ret_type F.tunit ret_type).
+  unfold arg_type.
+  unfold ret_type.
   constructor.
   simpl.
-  Qed.
+  constructor.
+  constructor.
+  constructor.
+  apply wtOm_tau.
+Qed.
 
 
-Definition case_uvalfi_tsum (n : nat) (τ1 τ2 : I.Ty) {P1 : ClosedTy τ1} {P2 : ClosedTy τ2} : F.Tm :=
-  let P := ClosedSum 0 P1 P2 in
-  let τ := @UValFI (S n) (I.tsum τ1 τ2) P in
-  let τ' := F.tsum (@UValFI n τ1 P1) (@UValFI n τ2 P2) in
+Definition case_uvalfi_tsum (n : nat) (τ1 τ2 : I.Ty) : F.Tm :=
+  let τ := UValFI (S n) (I.tsum τ1 τ2) in
+  let τ' := F.tsum (UValFI n τ1) (@UValFI n τ2) in
   let t := F.caseof (F.var 0) (F.var 0) (F.Om τ') in
   F.abs τ t.
 
-Definition case_uvalfi_trec (n : nat) (τb : I.Ty) {Pb : ClosedNTy 1 τb} : F.Tm :=
+Definition case_uvalfi_trec (n : nat) (τb : I.Ty) : F.Tm :=
   let τ_rec := I.trec τb in
-  let P := ClosedRec 0 Pb in
-  let P_unf := closed_rec_implies_closed_unfold P in
-  let τ := @UValFI (S n) τ_rec P in
-  let τ' := @UValFI n τb[beta1 τ_rec] P_unf in
+  let τ := UValFI (S n) τ_rec in
+  let τ' := UValFI n τb[beta1 τ_rec] in
   let t := F.caseof (F.var 0) (F.var 0) (F.Om τ') in
   F.abs τ t.
 
-Definition caseV0 (case₁ : Tm) (case₂ : Tm) :=
-  caseof (var 0) (case₁ [wkm↑]) (case₂[wkm↑]).
+Definition caseV0 (case₁ : F.Tm) (case₂ : F.Tm) : F.Tm :=
+  F.caseof (F.var 0) (case₁ [wkm↑]) (case₂[wkm↑]).
 
-Lemma caseV0_T {Γ τ₁ τ₂ τ case₁ case₂} :
-  ⟪ Γ ▻ τ₁ ⊢ case₁ : τ ⟫ →
-  ⟪ Γ ▻ τ₂ ⊢ case₂ : τ ⟫ →
-  ⟪ Γ ▻ (τ₁ ⊎ τ₂) ⊢ caseV0 case₁ case₂ : τ ⟫.
+Lemma caseV0_T {Γ : F.Env} {τ₁ τ₂ τ : F.Ty} {case₁ case₂ : F.Tm} :
+  F.Typing (F.evar Γ τ₁) case₁ τ →
+  F.Typing (F.evar Γ τ₂) case₂ τ →
+  F.Typing (F.evar Γ (F.tsum τ₁ τ₂)) (caseV0 case₁ case₂) τ.
 Proof.
   unfold caseV0.
-  crushTyping.
+  F.crushTyping.
 Qed.
 
 Hint Resolve caseV0_T : uval_typing.
 
-Definition caseUVal_pctx (tunk tcunit tcbool tcprod tcsum tcarr : Tm) : PCtx :=
-  pcaseof₁ phole
+Definition caseUVal_pctx (tunk tcunit tcbool tcprod tcsum tcarr : F.Tm) : F.PCtx :=
+  F.pcaseof₁ F.phole
          (tunk [wkm])
          (caseV0 tcunit
                  (caseV0 tcbool
                          (caseV0 tcprod
                                  (caseV0 tcarr tcsum)))).
-Definition caseUVal (tscrut tunk tcunit tcbool tcprod tcsum tcarr : Tm) :=
-  pctx_app tscrut (caseUVal_pctx tunk tcunit tcbool tcprod tcsum tcarr).
+Definition caseUVal (tscrut tunk tcunit tcbool tcprod tcsum tcarr : F.Tm) :=
+  F.pctx_app tscrut (caseUVal_pctx tunk tcunit tcbool tcprod tcsum tcarr).
 
 Arguments caseUVal tscrut tunk tcunit tcbool tcprod tcsum tcarr : simpl never.
 
-Lemma caseUVal_pctx_T {Γ n tunk tcunit tcbool tcprod tcsum tcarr τ} :
-  ⟪ Γ ⊢ tunk : τ ⟫ →
-  ⟪ Γ ▻ tunit ⊢ tcunit : τ ⟫ →
-  ⟪ Γ ▻ tbool ⊢ tcbool : τ ⟫ →
-  ⟪ Γ ▻ (UVal n × UVal n) ⊢ tcprod : τ ⟫ →
-  ⟪ Γ ▻ (UVal n ⊎ UVal n) ⊢ tcsum : τ ⟫ →
-  ⟪ Γ ▻ (UVal n ⇒ UVal n) ⊢ tcarr : τ ⟫ →
-  ⟪ ⊢ caseUVal_pctx tunk tcunit tcbool tcprod tcsum tcarr : Γ , UVal (S n) → Γ , τ ⟫.
-Proof.
-  unfold caseUVal_pctx. 
-  crushTyping.
-  eauto with typing uval_typing.
-Qed.
+(* Lemma caseUVal_pctx_T {Γ n tunk tcunit tcbool tcprod tcsum tcarr τ} : *)
+(*   ⟪ Γ ⊢ tunk : τ ⟫ → *)
+(*   ⟪ Γ ▻ tunit ⊢ tcunit : τ ⟫ → *)
+(*   ⟪ Γ ▻ tbool ⊢ tcbool : τ ⟫ → *)
+(*   (* ⟪ Γ ▻ (UVal n × UVal n) ⊢ tcprod : τ ⟫ → *) *)
+(*   ⟪ Γ ▻ (UVal n ⊎ UVal n) ⊢ tcsum : τ ⟫ → *)
+(*   ⟪ Γ ▻ (UVal n ⇒ UVal n) ⊢ tcarr : τ ⟫ → *)
+(*   ⟪ ⊢ caseUVal_pctx tunk tcunit tcbool tcprod tcsum tcarr : Γ , UVal (S n) → Γ , τ ⟫. *)
+(* Proof. *)
+(*   unfold caseUVal_pctx.  *)
+(*   crushTyping. *)
+(*   eauto with typing uval_typing. *)
+(* Qed. *)
 
 
-Lemma caseUVal_T {Γ n tscrut tunk tcunit tcbool tcprod tcsum tcarr τ} :
-  ⟪ Γ ⊢ tscrut : UVal (S n) ⟫ →
-  ⟪ Γ ⊢ tunk : τ ⟫ →
-  ⟪ Γ ▻ tunit ⊢ tcunit : τ ⟫ →
-  ⟪ Γ ▻ tbool ⊢ tcbool : τ ⟫ →
-  ⟪ Γ ▻ (UVal n × UVal n) ⊢ tcprod : τ ⟫ →
-  ⟪ Γ ▻ (UVal n ⊎ UVal n) ⊢ tcsum : τ ⟫ →
-  ⟪ Γ ▻ (UVal n ⇒ UVal n) ⊢ tcarr : τ ⟫ →
-  ⟪ Γ ⊢ caseUVal tscrut tunk tcunit tcbool tcprod tcsum tcarr : τ ⟫.
-Proof.
-  unfold caseUVal. 
-  eauto using caseUVal_pctx_T with typing.
-Qed.
+(* Lemma caseUVal_T {Γ n tscrut tunk tcunit tcbool tcprod tcsum tcarr τ} : *)
+(*   ⟪ Γ ⊢ tscrut : UVal (S n) ⟫ → *)
+(*   ⟪ Γ ⊢ tunk : τ ⟫ → *)
+(*   ⟪ Γ ▻ tunit ⊢ tcunit : τ ⟫ → *)
+(*   ⟪ Γ ▻ tbool ⊢ tcbool : τ ⟫ → *)
+(*   ⟪ Γ ▻ (UVal n × UVal n) ⊢ tcprod : τ ⟫ → *)
+(*   ⟪ Γ ▻ (UVal n ⊎ UVal n) ⊢ tcsum : τ ⟫ → *)
+(*   ⟪ Γ ▻ (UVal n ⇒ UVal n) ⊢ tcarr : τ ⟫ → *)
+(*   ⟪ Γ ⊢ caseUVal tscrut tunk tcunit tcbool tcprod tcsum tcarr : τ ⟫. *)
+(* Proof. *)
+(*   unfold caseUVal.  *)
+(*   eauto using caseUVal_pctx_T with typing. *)
+(* Qed. *)
 
-Arguments UVal n : simpl never.
+Arguments UValFI n : simpl never.
 Hint Resolve unkUValT : uval_typing.
-Hint Resolve inUnitT : uval_typing.
-Hint Resolve inBoolT : uval_typing.
-Hint Resolve inProd_T : uval_typing.
-Hint Resolve inSum_T : uval_typing.
-Hint Resolve inArr_T : uval_typing.
-Hint Resolve inUnit_pctx_T : uval_typing.
-Hint Resolve inBool_pctx_T : uval_typing.
-Hint Resolve inProd_pctx_T : uval_typing.
-Hint Resolve inSum_pctx_T : uval_typing.
-Hint Resolve inArr_pctx_T : uval_typing.
-Hint Resolve caseUVal_pctx_T : uval_typing.
-Hint Resolve caseUVal_T : uval_typing.
+(* Hint Resolve inUnitT : uval_typing. *)
+(* Hint Resolve inBoolT : uval_typing. *)
+(* Hint Resolve inProd_T : uval_typing. *)
+(* Hint Resolve inSum_T : uval_typing. *)
+(* Hint Resolve inArr_T : uval_typing. *)
+(* Hint Resolve inUnit_pctx_T : uval_typing. *)
+(* Hint Resolve inBool_pctx_T : uval_typing. *)
+(* Hint Resolve inProd_pctx_T : uval_typing. *)
+(* Hint Resolve inSum_pctx_T : uval_typing. *)
+(* Hint Resolve inArr_pctx_T : uval_typing. *)
+(* Hint Resolve caseUVal_pctx_T : uval_typing. *)
+(* Hint Resolve caseUVal_T : uval_typing. *)
 
 Local Ltac crush :=
   repeat (subst*;
@@ -321,346 +317,349 @@ Local Ltac crush :=
           repeat match goal with
                      [ |- _ ∧ _ ] => split
                  end;
-          trivial; 
+          trivial;
           eauto with ws typing uval_typing eval
          ).
 
-Lemma caseV0_eval_inl {v case₁ case₂}:
-  Value v →
-  (caseV0 case₁ case₂)[beta1 (inl v)] --> case₁ [beta1 v].
+Lemma caseV0_eval_inl {v case₁ case₂ : F.Tm}:
+  F.Value v →
+  F.eval (caseV0 case₁ case₂)[beta1 (F.inl v)] (case₁ [beta1 v]).
 Proof.
   intros vv.
-  unfold caseV0; apply eval₀_to_eval; crush.
-  change ((caseof (var 0) case₁[wkm↑] case₂ [wkm↑])[beta1 (inl v)]) with
-  (caseof (inl v) (case₁[wkm↑][(beta1 (inl v))↑]) (case₂[wkm↑][(beta1 (inl v))↑])).
+  unfold caseV0; apply F.eval₀_to_eval; crush.
+  change ((F.caseof (F.var 0) case₁[wkm↑] case₂ [wkm↑])[beta1 (F.inl v)]) with
+  (F.caseof (F.inl v) (case₁[wkm↑][(beta1 (F.inl v))↑]) (case₂[wkm↑][(beta1 (F.inl v))↑])).
   crush.
 Qed.
 
-Lemma caseV0_eval_inr {v case₁ case₂}:
-  Value v →
-  (caseV0 case₁ case₂)[beta1 (inr v)] --> case₂ [beta1 v].
+Lemma caseV0_eval_inr {v case₁ case₂ : F.Tm}:
+  F.Value v →
+  F.eval (caseV0 case₁ case₂)[beta1 (F.inr v)] (case₂ [beta1 v]).
 Proof.
   intros vv.
-  unfold caseV0; apply eval₀_to_eval; crush.
-  change ((caseof (var 0) case₁[wkm↑] case₂ [wkm↑])[beta1 (inr v)]) with
-  (caseof (inr v) (case₁[wkm↑][(beta1 (inr v))↑]) (case₂[wkm↑][(beta1 (inr v))↑])).
+  unfold caseV0; apply F.eval₀_to_eval; crush.
+  change ((F.caseof (F.var 0) case₁[wkm↑] case₂ [wkm↑])[beta1 (F.inr v)]) with
+  (F.caseof (F.inr v) (case₁[wkm↑][(beta1 (F.inr v))↑]) (case₂[wkm↑][(beta1 (F.inr v))↑])).
   crush.
 Qed.
 
 Lemma caseV0_eval {v τ₁ τ₂ case₁ case₂}:
-  Value v → ⟪ empty ⊢ v : τ₁ ⊎ τ₂ ⟫ →
-  (exists v', v = inl v' ∧ (caseV0 case₁ case₂)[beta1 v] --> case₁ [beta1 v']) ∨
-  (exists v', v = inr v' ∧ (caseV0 case₁ case₂)[beta1 v] --> case₂ [beta1 v']).
+  F.Value v → F.Typing F.empty v (F.tsum τ₁ τ₂) →
+  (exists v', v = F.inl v' ∧ F.eval (caseV0 case₁ case₂)[beta1 v] case₁[beta1 v']) ∨
+  (exists v', v = F.inr v' ∧ F.eval (caseV0 case₁ case₂)[beta1 v] case₂[beta1 v']).
 Proof.
   intros vv ty.
-  stlcCanForm; [left|right]; exists x; 
+  F.stlcCanForm; [left|right]; exists x;
   crush; eauto using caseV0_eval_inl, caseV0_eval_inr.
 Qed.
 
 Local Ltac crushEvalsInCaseUVal :=
-  repeat 
+  repeat
     (match goal with
-         [ |- caseof (inl _) _ _ -->* _ ] => (eapply (evalStepStar _); [eapply eval₀_to_eval; crush|])
-       | [ |- caseof (inr _) _ _ -->* _ ] => (eapply (evalStepStar _); [eapply eval₀_to_eval; crush|])
-       | [ |- (caseV0 _ _) [beta1 (inl _)] -->* _ ] => (eapply (evalStepStar _); [eapply caseV0_eval_inl; crush|])
-       | [ |- (caseV0 _ _) [beta1 (inr _)] -->* _ ] => (eapply (evalStepStar _); [eapply caseV0_eval_inr; crush|])
-       | [ |- ?t -->* ?t ] => eauto with eval
+         [ |- (F.horrible_thing (F.caseof (F.inl _) _ _) _) ] => (eapply (evalStepStar _); [eapply F.eval₀_to_eval; crush|])
+       | [ |- (F.horrible_thing (F.caseof (F.inr _) _ _) _) ] => (eapply (evalStepStar _); [eapply F.eval₀_to_eval; crush|])
+       | [ |- (F.horrible_thing ((caseV0 _ _) [beta1 (F.inl _)]) _) ] => (eapply (evalStepStar _); [eapply caseV0_eval_inl; crush|])
+       | [ |- (F.horrible_thing ((caseV0 _ _) [beta1 (F.inr _)]) _) ] => (eapply (evalStepStar _); [eapply caseV0_eval_inr; crush|])
+       | [ |- (F.horrible_thing ?t ?t) ] => eauto with *
      end;
      try rewrite -> apply_wkm_beta1_cancel
     ).
 
-Lemma canonUValS {n v} :
-  ⟪ empty ⊢ v : UVal (S n) ⟫ → Value v →
-  (v = unkUVal (S n)) ∨
-  (∃ v', v = inUnit n v' ∧ Value v' ∧ ⟪ empty ⊢ v' : tunit ⟫) ∨
-  (∃ v', v = inBool n v' ∧ Value v' ∧ ⟪ empty ⊢ v' : tbool ⟫) ∨
-  (∃ v', v = inProd n v' ∧ Value v' ∧ ⟪ empty ⊢ v' : UVal n × UVal n ⟫) ∨
-  (∃ v', v = inSum n v' ∧ Value v' ∧ ⟪ empty ⊢ v' : UVal n ⊎ UVal n ⟫) ∨
-  (∃ v', v = inArr n v' ∧ Value v' ∧ ⟪ empty ⊢ v' : UVal n ⇒ UVal n ⟫).
-Proof.
-  intros ty vv.
-  unfold UVal in ty; simpl. 
-  (* Apply canonical form lemmas but only as far as we need. *)
-  stlcCanForm1; 
-    [left|right;stlcCanForm1;
-       [left|right;stlcCanForm1;
-          [left|right;stlcCanForm1;
-                [left|right;stlcCanForm1;
-                      [right|left]]]]]. 
-  - stlcCanForm; crush.
-  - exists x0; crush.
-  - exists x; crush.
-  - exists x0; crush.
-  - exists x; crush.
-  - exists x; crush.
-Qed. 
+(* NOTE: for compatibility lemmas, we might need a UVal context and accompanying lemmas *)
 
-Lemma canonUVal {n v} :
-  ⟪ empty ⊢ v : UVal n ⟫ → Value v →
-  (v = unkUVal n) ∨
-  ∃ n', n = S n' ∧ 
-        ((∃ v', v = inUnit n' v' ∧ Value v' ∧ ⟪ empty ⊢ v' : tunit ⟫) ∨
-         (∃ v', v = inBool n' v' ∧ Value v' ∧ ⟪ empty ⊢ v' : tbool ⟫) ∨
-         (∃ v', v = inProd n' v' ∧ Value v' ∧ ⟪ empty ⊢ v' : UVal n' × UVal n' ⟫) ∨
-         (∃ v', v = inSum n' v' ∧ Value v' ∧ ⟪ empty ⊢ v' : UVal n' ⊎ UVal n' ⟫) ∨
-         (∃ v', v = inArr n' v' ∧ Value v' ∧ ⟪ empty ⊢ v' : UVal n' ⇒ UVal n' ⟫)).
-Proof.
-  intros ty vv.
-  destruct n.
-  - left. unfold UVal, unkUVal in *. stlcCanForm. trivial.
-  - destruct (canonUValS ty vv) as [? | ?].
-    + left; crush.
-    + right; crush. 
-Qed.
+(* Lemma canonUValS {n v} : *)
+(*   ⟪ empty ⊢ v : UVal (S n) ⟫ → Value v → *)
+(*   (v = unkUVal (S n)) ∨ *)
+(*   (∃ v', v = inUnit n v' ∧ Value v' ∧ ⟪ empty ⊢ v' : tunit ⟫) ∨ *)
+(*   (∃ v', v = inBool n v' ∧ Value v' ∧ ⟪ empty ⊢ v' : tbool ⟫) ∨ *)
+(*   (∃ v', v = inProd n v' ∧ Value v' ∧ ⟪ empty ⊢ v' : UVal n × UVal n ⟫) ∨ *)
+(*   (∃ v', v = inSum n v' ∧ Value v' ∧ ⟪ empty ⊢ v' : UVal n ⊎ UVal n ⟫) ∨ *)
+(*   (∃ v', v = inArr n v' ∧ Value v' ∧ ⟪ empty ⊢ v' : UVal n ⇒ UVal n ⟫). *)
+(* Proof. *)
+(*   intros ty vv. *)
+(*   unfold UVal in ty; simpl. *)
+(*   (* Apply canonical form lemmas but only as far as we need. *) *)
+(*   stlcCanForm1; *)
+(*     [left|right;stlcCanForm1; *)
+(*        [left|right;stlcCanForm1; *)
+(*           [left|right;stlcCanForm1; *)
+(*                 [left|right;stlcCanForm1; *)
+(*                       [right|left]]]]]. *)
+(*   - stlcCanForm; crush. *)
+(*   - exists x0; crush. *)
+(*   - exists x; crush. *)
+(*   - exists x0; crush. *)
+(*   - exists x; crush. *)
+(*   - exists x; crush. *)
+(* Qed. *)
 
-Ltac canonUVal :=
-  match goal with
-      [ H : Value ?v, H' : ⟪ empty ⊢ ?v : UVal 0 ⟫ |- _ ] =>
-      (unfold UVal in H'; stlcCanForm; subst)
-    | [ H : Value ?v, H' : ⟪ empty ⊢ ?v : UVal (S _) ⟫ |- _ ] =>
-      (destruct (canonUValS H' H) as 
-          [?| [(? & ? & ? & ?)
-              |[(? & ? & ? & ?)
-               |[(? & ? & ? & ?)
-                |[(? & ? & ? & ?)
-                 |(? & ? & ? & ?)]]]]]; subst)
-    | [ H : Value ?v, H' : ⟪ empty ⊢ ?v : UVal (S _ + _) ⟫ |- _ ] =>
-      (destruct (canonUValS H' H) as 
-          [?| [(? & ? & ? & ?)
-              |[(? & ? & ? & ?)
-               |[(? & ? & ? & ?)
-                |[(? & ? & ? & ?)
-                 |(? & ? & ? & ?)]]]]]; subst)
-    | [ H : Value ?v, H' : ⟪ empty ⊢ ?v : UVal _ ⟫ |- _ ] =>
-      (destruct (canonUVal H' H) as 
-          [?| (? & ? & [(? & ? & ? & ?)
-                       |[(? & ? & ? & ?)
-                        |[(? & ? & ? & ?)
-                         |[(? & ? & ? & ?)
-                          |(? & ? & ? & ?)]]]])]; subst)
-  end.
+(* Lemma canonUVal {n v} : *)
+(*   ⟪ empty ⊢ v : UVal n ⟫ → Value v → *)
+(*   (v = unkUVal n) ∨ *)
+(*   ∃ n', n = S n' ∧  *)
+(*         ((∃ v', v = inUnit n' v' ∧ Value v' ∧ ⟪ empty ⊢ v' : tunit ⟫) ∨ *)
+(*          (∃ v', v = inBool n' v' ∧ Value v' ∧ ⟪ empty ⊢ v' : tbool ⟫) ∨ *)
+(*          (∃ v', v = inProd n' v' ∧ Value v' ∧ ⟪ empty ⊢ v' : UVal n' × UVal n' ⟫) ∨ *)
+(*          (∃ v', v = inSum n' v' ∧ Value v' ∧ ⟪ empty ⊢ v' : UVal n' ⊎ UVal n' ⟫) ∨ *)
+(*          (∃ v', v = inArr n' v' ∧ Value v' ∧ ⟪ empty ⊢ v' : UVal n' ⇒ UVal n' ⟫)). *)
+(* Proof. *)
+(*   intros ty vv. *)
+(*   destruct n. *)
+(*   - left. unfold UVal, unkUVal in *. stlcCanForm. trivial. *)
+(*   - destruct (canonUValS ty vv) as [? | ?]. *)
+(*     + left; crush. *)
+(*     + right; crush.  *)
+(* Qed. *)
 
-Lemma caseUVal_eval_unk {n tunk tcunit tcbool tcprod tcsum tcarr} :
-  caseUVal (unkUVal (S n)) tunk tcunit tcbool tcprod tcsum tcarr -->* tunk.
-Proof.
-  unfold caseUVal, unkUVal; simpl.
-  (* why doesn't crush do the following? *)
-  assert (Value (inl unit)) by (simpl; trivial).
-  crushEvalsInCaseUVal.
-Qed.
-  
-Lemma caseUVal_eval_unit {n tunk tcunit tcbool tcprod tcsum tcarr v} :
-  Value v →
-  caseUVal (inUnit n v) tunk tcunit tcbool tcprod tcsum tcarr -->* tcunit [beta1 v].
-Proof.
-  intros vv.
-  unfold caseUVal, inUnit; simpl.
-  crushEvalsInCaseUVal.
-Qed.
-  
-Lemma caseUVal_eval_bool {n tunk tcunit tcbool tcprod tcsum tcarr v} :
-  Value v →
-  caseUVal (inBool n v) tunk tcunit tcbool tcprod tcsum tcarr -->* tcbool [beta1 v].
-Proof.
-  intros vv.
-  unfold caseUVal, inBool; simpl.
-  crushEvalsInCaseUVal.
-Qed.
-  
-Lemma caseUVal_eval_prod {n tunk tcunit tcbool tcprod tcsum tcarr v} :
-  Value v →
-  caseUVal (inProd n v) tunk tcunit tcbool tcprod tcsum tcarr -->* tcprod [beta1 v].
-Proof.
-  intros vv.
-  unfold caseUVal, inProd; simpl.
-  crushEvalsInCaseUVal.
-Qed.
+(* Ltac canonUVal := *)
+(*   match goal with *)
+(*       [ H : Value ?v, H' : ⟪ empty ⊢ ?v : UVal 0 ⟫ |- _ ] => *)
+(*       (unfold UVal in H'; stlcCanForm; subst) *)
+(*     | [ H : Value ?v, H' : ⟪ empty ⊢ ?v : UVal (S _) ⟫ |- _ ] => *)
+(*       (destruct (canonUValS H' H) as  *)
+(*           [?| [(? & ? & ? & ?) *)
+(*               |[(? & ? & ? & ?) *)
+(*                |[(? & ? & ? & ?) *)
+(*                 |[(? & ? & ? & ?) *)
+(*                  |(? & ? & ? & ?)]]]]]; subst) *)
+(*     | [ H : Value ?v, H' : ⟪ empty ⊢ ?v : UVal (S _ + _) ⟫ |- _ ] => *)
+(*       (destruct (canonUValS H' H) as  *)
+(*           [?| [(? & ? & ? & ?) *)
+(*               |[(? & ? & ? & ?) *)
+(*                |[(? & ? & ? & ?) *)
+(*                 |[(? & ? & ? & ?) *)
+(*                  |(? & ? & ? & ?)]]]]]; subst) *)
+(*     | [ H : Value ?v, H' : ⟪ empty ⊢ ?v : UVal _ ⟫ |- _ ] => *)
+(*       (destruct (canonUVal H' H) as  *)
+(*           [?| (? & ? & [(? & ? & ? & ?) *)
+(*                        |[(? & ? & ? & ?) *)
+(*                         |[(? & ? & ? & ?) *)
+(*                          |[(? & ? & ? & ?) *)
+(*                           |(? & ? & ? & ?)]]]])]; subst) *)
+(*   end. *)
 
-Lemma caseUVal_eval_sum {n tunk tcunit tcbool tcprod tcsum tcarr v} :
-  Value v →
-  caseUVal (inSum n v) tunk tcunit tcbool tcprod tcsum tcarr -->* tcsum [beta1 v].
-Proof.
-  intros vv.
-  unfold caseUVal, inSum; simpl.
-  crushEvalsInCaseUVal.
-Qed.
+(* Lemma caseUVal_eval_unk {n : nat} {tunk tcunit tcbool tcprod tcsum tcarr : F.Tm} : *)
+(*   F.horrible_thing (caseUVal (F.inr F.unit) tunk tcunit tcbool tcprod tcsum tcarr) tunk. *)
+(* Proof. *)
+(*   unfold caseUVal, unkUVal; simpl. *)
+(*   (* why doesn't crush do the following? *) *)
+(*   assert (Value (inl unit)) by (simpl; trivial). *)
+(*   crushEvalsInCaseUVal. *)
+(*   eauto with *. *)
+(* Qed. *)
 
-Lemma caseUVal_eval_arr {n tunk tcunit tcbool tcprod tcsum tcarr v} :
-  Value v →
-  caseUVal (inArr n v) tunk tcunit tcbool tcprod tcsum tcarr -->* tcarr [beta1 v].
-Proof.
-  intros vv.
-  unfold caseUVal, inArr; simpl.
-  crushEvalsInCaseUVal.
-Qed.
+(* Lemma caseUVal_eval_unit {n tunk tcunit tcbool tcprod tcsum tcarr v} : *)
+(*   Value v → *)
+(*   caseUVal (inUnit n v) tunk tcunit tcbool tcprod tcsum tcarr -->* tcunit [beta1 v]. *)
+(* Proof. *)
+(*   intros vv. *)
+(*   unfold caseUVal, inUnit; simpl. *)
+(*   crushEvalsInCaseUVal. *)
+(* Qed. *)
 
-Lemma caseUVal_sub {t tunk tcunit tcbool tcprod tcsum tcarr} γ :
-  (caseUVal t tunk tcunit tcbool tcprod tcsum tcarr)[γ] =
-  caseUVal (t[γ]) (tunk[γ]) (tcunit[γ↑]) (tcbool[γ↑]) (tcprod[γ↑]) (tcsum[γ↑]) (tcarr[γ↑]).
-Proof.
-  unfold caseUVal, caseUVal_pctx, caseV0. cbn. 
-  crush; 
-    rewrite <- ?apply_wkm_comm, <- ?(apply_wkm_up_comm); 
-    reflexivity.
-Qed.  
+(* Lemma caseUVal_eval_bool {n tunk tcunit tcbool tcprod tcsum tcarr v} : *)
+(*   Value v → *)
+(*   caseUVal (inBool n v) tunk tcunit tcbool tcprod tcsum tcarr -->* tcbool [beta1 v]. *)
+(* Proof. *)
+(*   intros vv. *)
+(*   unfold caseUVal, inBool; simpl. *)
+(*   crushEvalsInCaseUVal. *)
+(* Qed. *)
+
+(* Lemma caseUVal_eval_prod {n tunk tcunit tcbool tcprod tcsum tcarr v} : *)
+(*   Value v → *)
+(*   caseUVal (inProd n v) tunk tcunit tcbool tcprod tcsum tcarr -->* tcprod [beta1 v]. *)
+(* Proof. *)
+(*   intros vv. *)
+(*   unfold caseUVal, inProd; simpl. *)
+(*   crushEvalsInCaseUVal. *)
+(* Qed. *)
+
+(* Lemma caseUVal_eval_sum {n tunk tcunit tcbool tcprod tcsum tcarr v} : *)
+(*   Value v → *)
+(*   caseUVal (inSum n v) tunk tcunit tcbool tcprod tcsum tcarr -->* tcsum [beta1 v]. *)
+(* Proof. *)
+(*   intros vv. *)
+(*   unfold caseUVal, inSum; simpl. *)
+(*   crushEvalsInCaseUVal. *)
+(* Qed. *)
+
+(* Lemma caseUVal_eval_arr {n tunk tcunit tcbool tcprod tcsum tcarr v} : *)
+(*   Value v → *)
+(*   caseUVal (inArr n v) tunk tcunit tcbool tcprod tcsum tcarr -->* tcarr [beta1 v]. *)
+(* Proof. *)
+(*   intros vv. *)
+(*   unfold caseUVal, inArr; simpl. *)
+(*   crushEvalsInCaseUVal. *)
+(* Qed. *)
+
+(* Lemma caseUVal_sub {t tunk tcunit tcbool tcprod tcsum tcarr} γ : *)
+(*   (caseUVal t tunk tcunit tcbool tcprod tcsum tcarr)[γ] = *)
+(*   caseUVal (t[γ]) (tunk[γ]) (tcunit[γ↑]) (tcbool[γ↑]) (tcprod[γ↑]) (tcsum[γ↑]) (tcarr[γ↑]). *)
+(* Proof. *)
+(*   unfold caseUVal, caseUVal_pctx, caseV0. cbn.  *)
+(*   crush;  *)
+(*     rewrite <- ?apply_wkm_comm, <- ?(apply_wkm_up_comm);  *)
+(*     reflexivity. *)
+(* Qed. *)
 
 
-Arguments caseUVal tscrut tunk tcunit tcbool tcprod tcsum tcarr : simpl never.
-Arguments caseUVal_pctx tunk tcunit tcbool tcprod tcsum tcarr : simpl never.
+(* Arguments caseUVal tscrut tunk tcunit tcbool tcprod tcsum tcarr : simpl never. *)
+(* Arguments caseUVal_pctx tunk tcunit tcbool tcprod tcsum tcarr : simpl never. *)
 
-Lemma caseUVal_pctx_ECtx {tunk tcunit tcbool tcprod tcsum tcarr} :
-  ECtx (caseUVal_pctx tunk tcunit tcbool tcprod tcsum tcarr).
-Proof.
-  simpl; trivial.
-Qed.
+(* Lemma caseUVal_pctx_ECtx {tunk tcunit tcbool tcprod tcsum tcarr} : *)
+(*   ECtx (caseUVal_pctx tunk tcunit tcbool tcprod tcsum tcarr). *)
+(* Proof. *)
+(*   simpl; trivial. *)
+(* Qed. *)
 
 
 (* Definition caseUVal (n : nat) (tscrut tunk tcunit tcbool tcprod tcsum tcarr : Tm) := *)
 
-Definition caseUnit_pctx := caseUVal_pctx (stlcOmega tunit) (var 0) (stlcOmega tunit) (stlcOmega tunit) (stlcOmega tunit) (stlcOmega tunit).
-Definition caseBool_pctx := caseUVal_pctx (stlcOmega tbool) (stlcOmega tbool) (var 0) (stlcOmega tbool) (stlcOmega tbool) (stlcOmega tbool).
-Definition caseProd_pctx n := caseUVal_pctx (stlcOmega (UVal n × UVal n)) (stlcOmega (UVal n × UVal n)) (stlcOmega (UVal n × UVal n)) (var 0) (stlcOmega (UVal n × UVal n)) (stlcOmega (UVal n × UVal n)).
-Definition caseSum_pctx n := caseUVal_pctx (stlcOmega (UVal n ⊎ UVal n)) (stlcOmega (UVal n ⊎ UVal n)) (stlcOmega (UVal n ⊎ UVal n)) (stlcOmega (UVal n ⊎ UVal n)) (var 0) (stlcOmega (UVal n ⊎ UVal n)).
-Definition caseArr_pctx n := caseUVal_pctx (stlcOmega (UVal n ⇒ UVal n)) (stlcOmega (UVal n ⇒ UVal n)) (stlcOmega (UVal n ⇒ UVal n)) (stlcOmega (UVal n ⇒ UVal n)) (stlcOmega (UVal n ⇒ UVal n)) (var 0).
-Definition caseUnit t := pctx_app t caseUnit_pctx.
-Definition caseBool t := pctx_app t caseBool_pctx.
-Definition caseProd n t := pctx_app t (caseProd_pctx n).
-Definition caseSum n t := pctx_app t (caseSum_pctx n).
-Definition caseArr n t := pctx_app t (caseArr_pctx n).
+(* Definition caseUnit_pctx := caseUVal_pctx (stlcOmega tunit) (var 0) (stlcOmega tunit) (stlcOmega tunit) (stlcOmega tunit) (stlcOmega tunit). *)
+(* Definition caseBool_pctx := caseUVal_pctx (stlcOmega tbool) (stlcOmega tbool) (var 0) (stlcOmega tbool) (stlcOmega tbool) (stlcOmega tbool). *)
+(* Definition caseProd_pctx n := caseUVal_pctx (stlcOmega (UVal n × UVal n)) (stlcOmega (UVal n × UVal n)) (stlcOmega (UVal n × UVal n)) (var 0) (stlcOmega (UVal n × UVal n)) (stlcOmega (UVal n × UVal n)). *)
+(* Definition caseSum_pctx n := caseUVal_pctx (stlcOmega (UVal n ⊎ UVal n)) (stlcOmega (UVal n ⊎ UVal n)) (stlcOmega (UVal n ⊎ UVal n)) (stlcOmega (UVal n ⊎ UVal n)) (var 0) (stlcOmega (UVal n ⊎ UVal n)). *)
+(* Definition caseArr_pctx n := caseUVal_pctx (stlcOmega (UVal n ⇒ UVal n)) (stlcOmega (UVal n ⇒ UVal n)) (stlcOmega (UVal n ⇒ UVal n)) (stlcOmega (UVal n ⇒ UVal n)) (stlcOmega (UVal n ⇒ UVal n)) (var 0). *)
+(* Definition caseUnit t := pctx_app t caseUnit_pctx. *)
+(* Definition caseBool t := pctx_app t caseBool_pctx. *)
+(* Definition caseProd n t := pctx_app t (caseProd_pctx n). *)
+(* Definition caseSum n t := pctx_app t (caseSum_pctx n). *)
+(* Definition caseArr n t := pctx_app t (caseArr_pctx n). *)
 
-Lemma caseUnit_pctx_ECtx : ECtx caseUnit_pctx.
-Proof.
-  simpl; trivial.
-Qed.
+(* Lemma caseUnit_pctx_ECtx : ECtx caseUnit_pctx. *)
+(* Proof. *)
+(*   simpl; trivial. *)
+(* Qed. *)
 
-Lemma caseBool_pctx_ECtx : ECtx caseBool_pctx.
-Proof.
-  simpl; trivial.
-Qed.
+(* Lemma caseBool_pctx_ECtx : ECtx caseBool_pctx. *)
+(* Proof. *)
+(*   simpl; trivial. *)
+(* Qed. *)
 
-Lemma caseProd_pctx_ECtx {n}: ECtx (caseProd_pctx n).
-Proof.
-  simpl; trivial.
-Qed.
+(* Lemma caseProd_pctx_ECtx {n}: ECtx (caseProd_pctx n). *)
+(* Proof. *)
+(*   simpl; trivial. *)
+(* Qed. *)
 
-Lemma caseSum_pctx_ECtx {n}: ECtx (caseSum_pctx n).
-Proof.
-  simpl; trivial.
-Qed.
+(* Lemma caseSum_pctx_ECtx {n}: ECtx (caseSum_pctx n). *)
+(* Proof. *)
+(*   simpl; trivial. *)
+(* Qed. *)
 
-Lemma caseArr_pctx_ECtx {n}: ECtx (caseArr_pctx n).
-Proof.
-  simpl; trivial.
-Qed.
+(* Lemma caseArr_pctx_ECtx {n}: ECtx (caseArr_pctx n). *)
+(* Proof. *)
+(*   simpl; trivial. *)
+(* Qed. *)
 
-Lemma caseUnit_sub {t γ} :
-  (caseUnit t) [γ] = caseUnit (t [γ]).
-Proof.
-  unfold caseUnit; crush.
-Qed.
+(* Lemma caseUnit_sub {t γ} : *)
+(*   (caseUnit t) [γ] = caseUnit (t [γ]). *)
+(* Proof. *)
+(*   unfold caseUnit; crush. *)
+(* Qed. *)
 
-Lemma caseBool_sub {t γ} :
-  caseBool t [γ] = caseBool (t [γ]).
-Proof.
-  unfold caseBool; crush.
-Qed.
+(* Lemma caseBool_sub {t γ} : *)
+(*   caseBool t [γ] = caseBool (t [γ]). *)
+(* Proof. *)
+(*   unfold caseBool; crush. *)
+(* Qed. *)
 
-Lemma caseProd_sub {n t γ} :
-  caseProd n t [γ] = caseProd n (t [γ]).
-Proof.
-  unfold caseProd; crush.
-Qed.
+(* Lemma caseProd_sub {n t γ} : *)
+(*   caseProd n t [γ] = caseProd n (t [γ]). *)
+(* Proof. *)
+(*   unfold caseProd; crush. *)
+(* Qed. *)
 
-Lemma caseSum_sub {n t γ} :
-  caseSum n t [γ] = caseSum n (t [γ]).
-Proof.
-  unfold caseSum; crush.
-Qed.
+(* Lemma caseSum_sub {n t γ} : *)
+(*   caseSum n t [γ] = caseSum n (t [γ]). *)
+(* Proof. *)
+(*   unfold caseSum; crush. *)
+(* Qed. *)
 
-Lemma caseArr_sub {n t γ} :
-  (caseArr n t) [γ] = caseArr n (t [γ]).
-Proof.
-  unfold caseArr; crush.
-Qed.
+(* Lemma caseArr_sub {n t γ} : *)
+(*   (caseArr n t) [γ] = caseArr n (t [γ]). *)
+(* Proof. *)
+(*   unfold caseArr; crush. *)
+(* Qed. *)
 
-(* Arguments caseUnit n t : simpl never. *)
-(* Arguments caseBool n t : simpl never. *)
-(* Arguments caseProd n t : simpl never. *)
-(* Arguments caseSum n t : simpl never. *)
-(* Arguments caseArr n t : simpl never. *)
+(* (* Arguments caseUnit n t : simpl never. *) *)
+(* (* Arguments caseBool n t : simpl never. *) *)
+(* (* Arguments caseProd n t : simpl never. *) *)
+(* (* Arguments caseSum n t : simpl never. *) *)
+(* (* Arguments caseArr n t : simpl never. *) *)
 
-Lemma caseUnit_pctx_T {Γ n} : 
-  ⟪ ⊢ caseUnit_pctx : Γ , UVal (S n) → Γ , tunit ⟫.
-Proof.
-  unfold caseUnit_pctx.
-  eauto with typing uval_typing.
-Qed.
+(* Lemma caseUnit_pctx_T {Γ n} :  *)
+(*   ⟪ ⊢ caseUnit_pctx : Γ , UVal (S n) → Γ , tunit ⟫. *)
+(* Proof. *)
+(*   unfold caseUnit_pctx. *)
+(*   eauto with typing uval_typing. *)
+(* Qed. *)
 
-Lemma caseUnit_T {Γ n t} : 
-  ⟪ Γ ⊢ t : UVal (S n) ⟫ → ⟪ Γ ⊢ caseUnit t : tunit ⟫.
-Proof.
-  unfold caseUnit.
-  eauto using caseUnit_pctx_T with typing.
-Qed.
+(* Lemma caseUnit_T {Γ n t} :  *)
+(*   ⟪ Γ ⊢ t : UVal (S n) ⟫ → ⟪ Γ ⊢ caseUnit t : tunit ⟫. *)
+(* Proof. *)
+(*   unfold caseUnit. *)
+(*   eauto using caseUnit_pctx_T with typing. *)
+(* Qed. *)
 
-Lemma caseBool_pctx_T {Γ n} : 
-  ⟪ ⊢ caseBool_pctx : Γ , UVal (S n) → Γ , tbool ⟫.
-Proof.
-  unfold caseBool_pctx.
-  eauto with typing uval_typing.
-Qed.
+(* Lemma caseBool_pctx_T {Γ n} :  *)
+(*   ⟪ ⊢ caseBool_pctx : Γ , UVal (S n) → Γ , tbool ⟫. *)
+(* Proof. *)
+(*   unfold caseBool_pctx. *)
+(*   eauto with typing uval_typing. *)
+(* Qed. *)
 
-Lemma caseBool_T {Γ n t} : 
-  ⟪ Γ ⊢ t : UVal (S n) ⟫ → ⟪ Γ ⊢ caseBool t : tbool ⟫.
-Proof.
-  unfold caseBool.
-  eauto using caseBool_pctx_T with typing.
-Qed.
+(* Lemma caseBool_T {Γ n t} :  *)
+(*   ⟪ Γ ⊢ t : UVal (S n) ⟫ → ⟪ Γ ⊢ caseBool t : tbool ⟫. *)
+(* Proof. *)
+(*   unfold caseBool. *)
+(*   eauto using caseBool_pctx_T with typing. *)
+(* Qed. *)
 
-Lemma caseProd_pctx_T {Γ n} : 
-  ⟪ ⊢ caseProd_pctx n : Γ , UVal (S n) → Γ , UVal n × UVal n ⟫.
-Proof.
-  unfold caseProd_pctx.
-  eauto with typing uval_typing.
-Qed.
+(* Lemma caseProd_pctx_T {Γ n} :  *)
+(*   ⟪ ⊢ caseProd_pctx n : Γ , UVal (S n) → Γ , UVal n × UVal n ⟫. *)
+(* Proof. *)
+(*   unfold caseProd_pctx. *)
+(*   eauto with typing uval_typing. *)
+(* Qed. *)
 
-Lemma caseProd_T {Γ n t} : 
-  ⟪ Γ ⊢ t : UVal (S n) ⟫ → ⟪ Γ ⊢ caseProd n t : UVal n × UVal n ⟫.
-Proof.
-  unfold caseProd.
-  eauto using caseProd_pctx_T with typing.
-Qed.
+(* Lemma caseProd_T {Γ n t} :  *)
+(*   ⟪ Γ ⊢ t : UVal (S n) ⟫ → ⟪ Γ ⊢ caseProd n t : UVal n × UVal n ⟫. *)
+(* Proof. *)
+(*   unfold caseProd. *)
+(*   eauto using caseProd_pctx_T with typing. *)
+(* Qed. *)
 
-Lemma caseSum_pctx_T {Γ n} : 
-  ⟪ ⊢ caseSum_pctx n : Γ , UVal (S n) → Γ , UVal n ⊎ UVal n ⟫.
-Proof.
-  unfold caseSum_pctx.
-  eauto with typing uval_typing.
-Qed.
+(* Lemma caseSum_pctx_T {Γ n} :  *)
+(*   ⟪ ⊢ caseSum_pctx n : Γ , UVal (S n) → Γ , UVal n ⊎ UVal n ⟫. *)
+(* Proof. *)
+(*   unfold caseSum_pctx. *)
+(*   eauto with typing uval_typing. *)
+(* Qed. *)
 
-Lemma caseSum_T {Γ n t} : 
-  ⟪ Γ ⊢ t : UVal (S n) ⟫ → ⟪ Γ ⊢ caseSum n t : UVal n ⊎ UVal n ⟫.
-Proof.
-  unfold caseSum.
-  eauto using caseSum_pctx_T with typing.
-Qed.
+(* Lemma caseSum_T {Γ n t} :  *)
+(*   ⟪ Γ ⊢ t : UVal (S n) ⟫ → ⟪ Γ ⊢ caseSum n t : UVal n ⊎ UVal n ⟫. *)
+(* Proof. *)
+(*   unfold caseSum. *)
+(*   eauto using caseSum_pctx_T with typing. *)
+(* Qed. *)
 
-Lemma caseArr_pctx_T {Γ n} : 
-  ⟪ ⊢ caseArr_pctx n : Γ , UVal (S n) → Γ , UVal n ⇒ UVal n ⟫.
-Proof.
-  unfold caseArr_pctx.
-  eauto with typing uval_typing.
-Qed.
+(* Lemma caseArr_pctx_T {Γ n} :  *)
+(*   ⟪ ⊢ caseArr_pctx n : Γ , UVal (S n) → Γ , UVal n ⇒ UVal n ⟫. *)
+(* Proof. *)
+(*   unfold caseArr_pctx. *)
+(*   eauto with typing uval_typing. *)
+(* Qed. *)
 
-Lemma caseArr_T {Γ n t} : 
-  ⟪ Γ ⊢ t : UVal (S n) ⟫ → ⟪ Γ ⊢ caseArr n t : UVal n ⇒ UVal n ⟫.
-Proof.
-  unfold caseArr.
-  eauto using caseArr_pctx_T with typing.
-Qed.
+(* Lemma caseArr_T {Γ n t} :  *)
+(*   ⟪ Γ ⊢ t : UVal (S n) ⟫ → ⟪ Γ ⊢ caseArr n t : UVal n ⇒ UVal n ⟫. *)
+(* Proof. *)
+(*   unfold caseArr. *)
+(*   eauto using caseArr_pctx_T with typing. *)
+(* Qed. *)
 
-Hint Resolve caseUnit_T : uval_typing.
-Hint Resolve caseBool_T : uval_typing.
-Hint Resolve caseProd_T : uval_typing.
-Hint Resolve caseSum_T : uval_typing.
-Hint Resolve caseArr_T : uval_typing.
+(* Hint Resolve caseUnit_T : uval_typing. *)
+(* Hint Resolve caseBool_T : uval_typing. *)
+(* Hint Resolve caseProd_T : uval_typing. *)
+(* Hint Resolve caseSum_T : uval_typing. *)
+(* Hint Resolve caseArr_T : uval_typing. *)
