FixIsMu/CompilerFI/CompilerFI.v
@@ -1,0 +1,318 @@
+(* Require Import StlcFix.SpecScoping. *)
+(* Require Import StlcFix.LemmasScoping. *)
+(* Require Import StlcFix.DecideEval. *)
+(* Require Import LogRel.PseudoType. *)
+(* Require Import LogRel.LemmasPseudoType. *)
+(* Require Import LogRel.LR. *)
+(* Require Import LogRel.LemmasLR. *)
+(* Require Import LogRel.LemmasIntro. *)
+Require Import Lia.
+Require Import Db.Lemmas.
+
+Require Import StlcFix.SpecEvaluation.
+Require Import StlcFix.SpecSyntax.
+Require Import StlcFix.SpecTyping.
+Require Import StlcFix.LemmasTyping.
+Require Import StlcFix.LemmasEvaluation.
+Require Import StlcFix.CanForm.
+
+Require Import StlcIso.SpecEvaluation.
+Require Import StlcIso.SpecSyntax.
+Require Import StlcIso.SpecTyping.
+Require Import StlcIso.LemmasTyping.
+Require Import StlcIso.LemmasEvaluation.
+Require Import StlcIso.CanForm.
+
+Module F.
+  Include StlcFix.SpecEvaluation.
+  Include StlcFix.SpecSyntax.
+  Include StlcFix.SpecTyping.
+  Include StlcFix.LemmasTyping.
+  Include StlcFix.LemmasEvaluation.
+  Include StlcFix.CanForm.
+End F.
+
+Module I.
+  Include StlcIso.SpecEvaluation.
+  Include StlcIso.SpecSyntax.
+  Include StlcIso.SpecTyping.
+  Include StlcIso.LemmasTyping.
+  Include StlcIso.LemmasEvaluation.
+  Include StlcIso.CanForm.
+End I.
+
+Fixpoint compfi_ty (τ : F.Ty) : I.Ty :=
+  match τ with
+    | F.tunit => I.tunit
+    | F.tarr τ1 τ2 => I.tarr (compfi_ty τ1) (compfi_ty τ2)
+    | F.tsum τ1 τ2 => I.tsum (compfi_ty τ1) (compfi_ty τ2)
+  end.
+
+Fixpoint compfi (t : F.Tm) : I.Tm :=
+  match t with
+    | F.var x => I.var x
+    | F.abs τ t => I.abs (compfi_ty τ) (compfi t)
+    | F.app t1 t2 => I.app (compfi t1) (compfi t2)
+    | F.unit => I.unit
+    | F.inl t => I.inl (compfi t)
+    | F.inr t => I.inr (compfi t)
+    | F.caseof t1 t2 t3 => I.caseof (compfi t1) (compfi t2) (compfi t3)
+    | F.fixt τ1 τ2 t =>
+      let fold_type := I.trec (I.tarr (I.tvar 0) (compfi_ty (F.tarr τ1 τ2))) in
+      let fny := I.abs (compfi_ty τ1) (I.app (I.app (I.unfold_ (I.var 1)) (I.var 1)) (I.var 0)) in
+      let fnx := I.abs fold_type (I.app (I.var 1) fny) in
+      let fnf := I.abs (compfi_ty (F.tarr (F.tarr τ1 τ2) (F.tarr τ1 τ2))) (I.app (fnx) (I.fold_ fnx)) in
+      I.app fnf (compfi t)
+  end.
+
+Lemma smoke_test_compiler :
+  (compfi F.unit) = I.unit.
+Proof.
+  simpl. reflexivity.
+Qed.
+
+(* Fixpoint erase (t : S.Tm) : U.UTm := *)
+(*   match t with *)
+(*     | S.abs τ t         => U.abs (erase t) *)
+(*     | S.unit            => U.unit *)
+(*     | S.true            => U.true *)
+(*     | S.false           => U.false *)
+(*     | S.pair t₁ t₂      => U.pair (erase t₁) (erase t₂) *)
+(*     | S.inl t           => U.inl (erase t) *)
+(*     | S.inr t           => U.inr (erase t) *)
+(*     | S.var x           => U.var x *)
+(*     | S.app t₁ t₂       => U.app (erase t₁) (erase t₂) *)
+(*     | S.ite t₁ t₂ t₃    => U.ite (erase t₁) (erase t₂) (erase t₃) *)
+(*     | S.proj₁ t₁        => U.proj₁ (erase t₁) *)
+(*     | S.proj₂ t₁        => U.proj₂ (erase t₁) *)
+(*     | S.caseof t₁ t₂ t₃ => U.caseof (erase t₁) (erase t₂) (erase t₃) *)
+(*     | S.seq t₁ t₂       => U.seq (erase t₁) (erase t₂) *)
+(*     | S.fixt _ _ t₁     => U.app U.ufix (erase t₁) *)
+(*   end. *)
+
+(* Fixpoint erase_pctx (C : S.PCtx) : U.PCtx := *)
+(*   match C with *)
+(*     | S.phole => phole *)
+(*     | S.pabs τ C => U.pabs (erase_pctx C) *)
+(*     | S.papp₁ C t => U.papp₁ (erase_pctx C) (erase t)  *)
+(*     | S.papp₂ t C => U.papp₂ (erase t) (erase_pctx C) *)
+(*     | S.pite₁ C t₂ t₃ => U.pite₁ (erase_pctx C) (erase t₂) (erase t₃) *)
+(*     | S.pite₂ t₁ C t₃ => U.pite₂ (erase t₁) (erase_pctx C) (erase t₃) *)
+(*     | S.pite₃ t₁ t₂ C => U.pite₃ (erase t₁) (erase t₂) (erase_pctx C) *)
+(*     | S.ppair₁ C t => U.ppair₁ (erase_pctx C) (erase t) *)
+(*     | S.ppair₂ t C => U.ppair₂ (erase t) (erase_pctx C) *)
+(*     | S.pproj₁ C => U.pproj₁ (erase_pctx C) *)
+(*     | S.pproj₂ C => U.pproj₂ (erase_pctx C) *)
+(*     | S.pinl C => U.pinl (erase_pctx C) *)
+(*     | S.pinr C => U.pinr (erase_pctx C) *)
+(*     | S.pcaseof₁ C t₂ t₃ => U.pcaseof₁ (erase_pctx C) (erase t₂) (erase t₃) *)
+(*     | S.pcaseof₂ t₁ C t₃ => U.pcaseof₂ (erase t₁) (erase_pctx C) (erase t₃) *)
+(*     | S.pcaseof₃ t₁ t₂ C => U.pcaseof₃ (erase t₁) (erase t₂) (erase_pctx C) *)
+(*     | S.pseq₁ C t => U.pseq₁ (erase_pctx C) (erase t) *)
+(*     | S.pseq₂ t C => U.pseq₂ (erase t) (erase_pctx C) *)
+(*     | S.pfixt τ₁ τ₂ C => U.papp₂ U.ufix (erase_pctx C) *)
+(*   end. *)
+
+(* Lemma erase_scope (t : S.Tm) (Γ : S.Env) (τ : S.Ty) : *)
+(*   ⟪ Γ ⊢ t : τ ⟫ -> ⟨ dom Γ ⊢ erase t ⟩. *)
+(* Proof. *)
+(*   intro wt; induction wt; crushUtlcScoping. *)
+(*   apply U.ufix_ws. *)
+(* Qed. *)
+
+(* Hint Extern 4 ⟨ _ ⊢ erase ?t ⟩ => *)
+(*   match goal with *)
+(*       [ H : ⟪ _ ⊢ ?t : _ ⟫ |- _ ] => refine (erase_scope _ _ _ H) *)
+(*   end. *)
+
+(* Lemma erase_pctx_scope (C : S.PCtx) (Γ₀ Γ : S.Env) (τ₀ τ : S.Ty) : *)
+(*   ⟪ ⊢ C : Γ₀ , τ₀ → Γ , τ ⟫ → ⟨ ⊢ erase_pctx C : dom Γ₀ → dom Γ ⟩. *)
+(* Proof. *)
+(*   intro wt; induction wt; crushUtlcScoping. *)
+(*   apply U.ufix_ws. *)
+(* Qed. *)
+
+(* Local Ltac crush := *)
+(*   cbn in * |- ; *)
+(*   repeat *)
+(*     (cbn; *)
+(*      repeat crushLRMatch; *)
+(*      crushOfType; *)
+(*      crushTyping; *)
+(*      repeat crushRepEmulEmbed; *)
+(*      repeat crushUtlcSyntaxMatchH; *)
+(*      repeat crushUtlcScopingMatchH; *)
+(*      subst; *)
+(*      trivial *)
+(*     ); try omega; eauto. *)
+
+(* Section CompatibilityLemmas. *)
+
+(*   Lemma compat_lambda {Γ τ' ts d n tu τ} : *)
+(*     ⟪ Γ p▻ τ' ⊩ ts ⟦ d , n ⟧ tu : τ ⟫ → *)
+(*     ⟪ Γ ⊩ (S.abs (repEmul τ') ts) ⟦ d , n ⟧ U.abs tu : ptarr τ' τ ⟫. *)
+(*   Proof. *)
+(*     crush. *)
+(*     - eauto using wsSub_up, envrel_implies_WsSub, wsAp. *)
+(*     - eauto using wtSub_up, envrel_implies_WtSub. *)
+(*     - rewrite -> ?ap_comp. *)
+(*       apply H1; crush. *)
+(*   Qed. *)
+
+(*   Lemma compat_lambda_embed {Γ τ' ts d n tu τ} : *)
+(*     ⟪ Γ p▻ embed τ' ⊩ ts ⟦ d , n ⟧ tu : τ ⟫ → *)
+(*     ⟪ Γ ⊩ (S.abs τ' ts) ⟦ d , n ⟧ abs tu : ptarr (embed τ') τ ⟫. *)
+(*   Proof. *)
+(*     rewrite <- (repEmul_embed_leftinv τ') at 2. *)
+(*     apply compat_lambda. *)
+(*   Qed. *)
+
+(*   Lemma compat_unit {Γ d n} : *)
+(*     ⟪ Γ ⊩ S.unit ⟦ d , n ⟧ U.unit : ptunit ⟫. *)
+(*   Proof. *)
+(*     crush. *)
+(*   Qed. *)
+
+(*   Lemma compat_true {Γ d n} : *)
+(*     ⟪ Γ ⊩ S.true ⟦ d , n ⟧ U.true : ptbool ⟫. *)
+(*   Proof. *)
+(*     crush. *)
+(*   Qed. *)
+
+(*   Lemma compat_false {Γ d n} : *)
+(*     ⟪ Γ ⊩ S.false ⟦ d , n ⟧ U.false : ptbool ⟫. *)
+(*   Proof. *)
+(*     crush. *)
+(*   Qed. *)
+
+(*   Lemma compat_pair {Γ d n ts₁ tu₁ τ₁ ts₂ tu₂ τ₂} : *)
+(*     ⟪ Γ ⊩ ts₁ ⟦ d , n ⟧ tu₁ : τ₁ ⟫ → *)
+(*     ⟪ Γ ⊩ ts₂ ⟦ d , n ⟧ tu₂ : τ₂ ⟫ → *)
+(*     ⟪ Γ ⊩ S.pair ts₁ ts₂ ⟦ d , n ⟧ U.pair tu₁ tu₂ : ptprod τ₁ τ₂ ⟫. *)
+(*   Proof. *)
+(*     crush. *)
+(*     apply termrel_pair; crush. *)
+(*     refine (H2 w' _ _ _ _); unfold lev in *; try omega. *)
+(*     eauto using envrel_mono. *)
+(*   Qed. *)
+
+(*   Lemma compat_app {Γ d n ts₁ tu₁ τ₁ ts₂ tu₂ τ₂} : *)
+(*     ⟪ Γ ⊩ ts₁ ⟦ d , n ⟧ tu₁ : ptarr τ₁ τ₂ ⟫ → *)
+(*     ⟪ Γ ⊩ ts₂ ⟦ d , n ⟧ tu₂ : τ₁ ⟫ → *)
+(*     ⟪ Γ ⊩ S.app ts₁ ts₂ ⟦ d , n ⟧ U.app tu₁ tu₂ : τ₂ ⟫. *)
+(*   Proof. *)
+(*     crush. *)
+(*     refine (termrel_app _ _); crush. *)
+(*     refine (H2 w' _ _ _ _); unfold lev in *; try omega. *)
+(*     crush. *)
+(*   Qed. *)
+
+(*   Lemma compat_inl {Γ d n ts tu τ₁ τ₂} : *)
+(*     ⟪ Γ ⊩ ts ⟦ d , n ⟧ tu : τ₁ ⟫ → *)
+(*     ⟪ Γ ⊩ S.inl ts ⟦ d , n ⟧ U.inl tu : ptsum τ₁ τ₂ ⟫. *)
+(*   Proof. *)
+(*     crush. *)
+(*     refine (termrel_inl _); crush. *)
+(*   Qed. *)
+
+(*   Lemma compat_inr {Γ d n ts tu τ₁ τ₂} : *)
+(*     ⟪ Γ ⊩ ts ⟦ d , n ⟧ tu : τ₂ ⟫ → *)
+(*     ⟪ Γ ⊩ S.inr ts ⟦ d , n ⟧ U.inr tu : ptsum τ₁ τ₂ ⟫. *)
+(*   Proof. *)
+(*     crush. *)
+(*     refine (termrel_inr _); crush. *)
+(*   Qed. *)
+
+(*   Lemma compat_seq {Γ d n ts₁ tu₁ ts₂ tu₂ τ₂} : *)
+(*     ⟪ Γ ⊩ ts₁ ⟦ d , n ⟧ tu₁ : ptunit ⟫ → *)
+(*     ⟪ Γ ⊩ ts₂ ⟦ d , n ⟧ tu₂ : τ₂ ⟫ → *)
+(*     ⟪ Γ ⊩ S.seq ts₁ ts₂ ⟦ d , n ⟧ U.seq tu₁ tu₂ : τ₂ ⟫. *)
+(*   Proof. *)
+(*     crush. *)
+(*     apply termrel_seq; crush. *)
+(*     refine (H2 w' _ _ _ _); crush. *)
+(*   Qed. *)
+
+(*   Lemma compat_proj₂ {Γ d n ts tu τ₁ τ₂} : *)
+(*     ⟪ Γ ⊩ ts ⟦ d , n ⟧ tu : ptprod τ₁ τ₂ ⟫ → *)
+(*     ⟪ Γ ⊩ S.proj₂ ts ⟦ d , n ⟧ U.proj₂ tu : τ₂ ⟫. *)
+(*   Proof. *)
+(*     crush. *)
+(*     refine (termrel_proj₂ _); crush. *)
+(*   Qed. *)
+
+(*   Lemma compat_proj₁ {Γ d n ts tu τ₁ τ₂} : *)
+(*     ⟪ Γ ⊩ ts ⟦ d , n ⟧ tu : ptprod τ₁ τ₂ ⟫ → *)
+(*     ⟪ Γ ⊩ S.proj₁ ts ⟦ d , n ⟧ U.proj₁ tu : τ₁ ⟫. *)
+(*   Proof. *)
+(*     crush. *)
+(*     refine (termrel_proj₁ _); crush. *)
+(*   Qed. *)
+
+(*   Lemma compat_ite {Γ d n ts₁ tu₁ ts₂ tu₂ ts₃ tu₃ τ} : *)
+(*     ⟪ Γ ⊩ ts₁ ⟦ d , n ⟧ tu₁ : ptbool ⟫ → *)
+(*     ⟪ Γ ⊩ ts₂ ⟦ d , n ⟧ tu₂ : τ ⟫ → *)
+(*     ⟪ Γ ⊩ ts₃ ⟦ d , n ⟧ tu₃ : τ ⟫ → *)
+(*     ⟪ Γ ⊩ S.ite ts₁ ts₂ ts₃ ⟦ d , n ⟧ U.ite tu₁ tu₂ tu₃ : τ ⟫. *)
+(*   Proof. *)
+(*     crush. *)
+(*     apply termrel_ite; crush. *)
+(*     - refine (H5 w' _ _ _ _); crush. *)
+(*     - refine (H3 w' _ _ _ _); crush. *)
+(*   Qed. *)
+
+(*   Lemma compat_caseof {Γ d n ts₁ tu₁ ts₂ tu₂ ts₃ tu₃ τ₁ τ₂ τ} : *)
+(*     ⟪ Γ ⊩ ts₁ ⟦ d , n ⟧ tu₁ : ptsum τ₁ τ₂ ⟫ → *)
+(*     ⟪ Γ p▻ τ₁ ⊩ ts₂ ⟦ d , n ⟧ tu₂ : τ ⟫ → *)
+(*     ⟪ Γ p▻ τ₂ ⊩ ts₃ ⟦ d , n ⟧ tu₃ : τ ⟫ → *)
+(*     ⟪ Γ ⊩ S.caseof ts₁ ts₂ ts₃ ⟦ d , n ⟧ U.caseof tu₁ tu₂ tu₃ : τ ⟫. *)
+(*   Proof. *)
+(*     crush. *)
+(*     refine (termrel_caseof _ _ _); crush; *)
+(*     rewrite -> ?ap_comp. *)
+(*     - refine (H5 w' _ _ _ _); crush. *)
+(*     - refine (H3 w' _ _ _ _); crush. *)
+(*   Qed. *)
+
+(*   Lemma compat_fix {Γ d n ts tu τ₁ τ₂} : *)
+(*     ⟪ Γ ⊩ ts ⟦ d , n ⟧ tu : ptarr (ptarr τ₁ τ₂) (ptarr τ₁ τ₂) ⟫ → *)
+(*     ⟪ Γ ⊩ S.fixt (repEmul τ₁) (repEmul τ₂) ts ⟦ d , n ⟧ U.app U.ufix tu : ptarr τ₁ τ₂ ⟫. *)
+(*   Proof. *)
+(*     crush. *)
+(*     - eapply ufix_ws. *)
+(*     - refine (termrel_fix _); crush. *)
+(*   Qed. *)
+
+(*   Lemma compat_fix' {Γ d n ts tu τ₁ τ₂} : *)
+(*     ⟪ Γ ⊩ ts ⟦ d , n ⟧ tu : embed (tarr (tarr τ₁ τ₂) (tarr τ₁ τ₂)) ⟫ → *)
+(*     ⟪ Γ ⊩ S.fixt τ₁ τ₂ ts ⟦ d , n ⟧ U.app U.ufix tu : ptarr (embed τ₁) (embed τ₂) ⟫. *)
+(*   Proof. *)
+(*     intros tr. *)
+(*     rewrite <- (repEmul_embed_leftinv τ₁) at 1. *)
+(*     rewrite <- (repEmul_embed_leftinv τ₂) at 1. *)
+(*     apply compat_fix; assumption. *)
+(*   Qed. *)
+
+(*   Lemma erase_correct {Γ d n ts τ} : *)
+(*     ⟪ Γ ⊢ ts : τ ⟫ → *)
+(*     ⟪ embedCtx Γ ⊩ ts ⟦ d , n ⟧ erase ts : embed τ ⟫. *)
+(*   Proof. *)
+(*     induction 1; simpl; eauto using compat_inl, compat_inr, compat_pair, compat_lambda_embed, compat_app, compat_false, compat_true, compat_var, compat_unit, embedCtx_works, compat_seq, compat_ite, compat_proj₁, compat_proj₂, compat_caseof, compat_fix'. *)
+(*   Qed.  *)
+
+(*   Lemma erase_ctx_correct {Γ Γ' d n C τ τ'} : *)
+(*     ⟪ ⊢ C : Γ , τ → Γ' , τ'⟫ → *)
+(*     ⟪ ⊩ C ⟦ d , n ⟧ erase_pctx C : embedCtx Γ , embed τ → embedCtx Γ' , embed τ' ⟫. *)
+(*   Proof. *)
+(*     intros ty; unfold OpenLRCtxN; split; [crush|idtac]. *)
+(*     induction ty; simpl;  *)
+(*     intros ts tu lr; *)
+(*       try assumption; (* deal with phole *) *)
+(*       repeat match goal with *)
+(*                | [ H : ⟪ _ ⊢ _ : _ ⟫ |- _ ] => eapply erase_correct in H *)
+(*              end; *)
+(*       specialize (IHty ts tu lr); *)
+(*       eauto using compat_inl, compat_inr, compat_pair, compat_lambda_embed, compat_app, compat_false, compat_true, compat_var, compat_unit, embedCtx_works, compat_seq, compat_ite, compat_proj₁, compat_proj₂, compat_caseof, compat_fix'. *)
+(*   Qed.  *)
+
+(* End CompatibilityLemmas. *)
