FixIsMu/LogRelFI/LRFI.v
@@ -1,0 +1,235 @@
+Require Export LogRel.PseudoType.
+Require Import LogRel.LemmasPseudoType.
+Require Import LogRel.PseudoType.
+Require Import StlcFix.SpecSyntax.
+Require Import StlcFix.SpecEvaluation.
+Require Import StlcFix.SpecTyping.
+Require Import StlcIso.SpecSyntax.
+Require Import StlcIso.SpecEvaluation.
+Require Import StlcIso.Inst.
+Require Import UVal.UVal.
+
+Require Import Coq.Program.Basics.
+Require Import Coq.Logic.FunctionalExtensionality.
+Require Import Coq.Arith.Wf_nat.
+Require Import Omega.
+
+Inductive Direction : Set :=
+| dir_lt
+| dir_gt.
+
+Definition World := nat.
+Definition lev : World → nat := fun w => w.
+Definition later : World → World := pred.
+Fixpoint lateri (i : nat) : World → World :=
+  match i with 
+    | 0 => id
+    | S i => fun w => pred (lateri i w)
+  end.
+
+Definition PTRel := PTy → S.Tm → U.UTm → Prop.
+Definition PCRel := PTy → S.PCtx → U.PCtx → Prop.
+
+(* Intuitively: observing termination takes a step in addition to the actual evaluation steps *)
+Definition Observe (n : nat) (T : nat → Prop) : Prop :=
+  match n with
+    | 0 => False
+    | S n' => T n'
+  end.
+
+Lemma lt_le {w w' w''} (fw : w' < w) (fw' : w'' ≤ w') : w'' < w.
+Proof.
+  unfold lt in *.
+  refine (le_trans _ _ _ _ fw).
+  refine (le_n_S _ _ fw').
+Defined.
+
+Definition prod_rel (R₁ R₂ : S.Tm → U.UTm → Prop) : S.Tm → U.UTm → Prop :=
+  fun ts tu =>
+    match ts , tu with
+      | S.pair ts₁ ts₂ , U.pair tu₁ tu₂ => R₁ ts₁ tu₁ ∧ R₂ ts₂ tu₂
+      | _              , _              => False
+    end.
+Definition sum_rel (R₁ R₂ : S.Tm → U.UTm → Prop) : S.Tm → U.UTm → Prop :=
+  fun ts tu =>
+    match ts , tu with
+      | S.inl ts' , U.inl tu' => R₁ ts' tu'
+      | S.inr ts' , U.inr tu' => R₂ ts' tu'
+      | _         , _         => False
+    end.
+Definition arr_rel (R₁ R₂ : S.Tm → U.UTm → Prop) : S.Tm → U.UTm → Prop :=
+  fun ts tu =>
+    match ts , tu with
+      | S.abs τ₁' tsb , U.abs tub =>
+        ∀ ts' tu',
+          R₁ ts' tu' →
+          R₂ (tsb [beta1 ts']) (tub [beta1 tu'])
+      | _ , _ => False
+    end.
+
+Arguments prod_rel R₁ R₂ !ts !tu.
+Arguments sum_rel R₁ R₂ !ts !tu.
+Arguments arr_rel R₁ R₂ !ts !tu.
+
+Section LogicalRelation.
+
+  Variable (d: Direction).
+
+  Definition Obs (w : World) (ts : S.Tm) (tu : U.UTm) :=
+    match d with
+      | dir_lt => Observe (lev w) (S.TerminatingN ts) → U.Terminating tu
+      | dir_gt => Observe (lev w) (U.TerminatingN tu) → S.Terminating ts
+    end.
+
+  Definition contrel' (w : World) (vr' : ∀ w' : World, w' ≤ w → PTRel) : PCRel :=
+   fun τ Cs Cu => ∀ w' (fw : w' ≤ w) ts tu, vr' w' fw τ ts tu → Obs w' (S.pctx_app ts Cs) (U.pctx_app tu Cu).
+
+  Definition termrel' (w : World) (vr' : ∀ w' : World, w' ≤ w → PTRel) : PTRel :=
+    fun τ ts tu => ∀ Cs Cu, S.ECtx Cs → U.ECtx Cu → contrel' w vr' τ Cs Cu → Obs w (S.pctx_app ts Cs) (U.pctx_app tu Cu).
+
+  Definition valrel' (w : World) (ind : ∀ w' : World, w' < w → PTRel) : PTRel :=
+    fun τ ts tu =>
+      OfType τ ts tu ∧
+      let latervr : PTRel := fun τ ts tu => ∀ w' (fw : w' < w), ind w' fw τ ts tu in
+      let laterlatervr : ∀ w' (fw : w' < w) w'' (fw' : w'' ≤ w'), PTRel := fun w' fw w'' fw' => ind w'' (lt_le fw fw') in
+      let vrunit : S.Tm → U.UTm → Prop := fun ts tu => ts = S.unit ∧ tu = U.unit in
+      let vrbool : S.Tm → U.UTm → Prop := fun ts tu => (ts = S.true ∧ tu = U.true) ∨ (ts = S.false ∧ tu = U.false) in
+      let vrprod : PTy → PTy → S.Tm → U.UTm → Prop :=
+          fun τ₁ τ₂ =>
+            prod_rel (latervr τ₁) (latervr τ₂) in
+      let vrsum : PTy → PTy → S.Tm → U.UTm → Prop :=
+          fun τ₁ τ₂ =>
+            sum_rel (latervr τ₁) (latervr τ₂) in
+      let vrarr : PTy → PTy → S.Tm → U.UTm → Prop :=
+          fun τ₁ τ₂ ts tu =>
+            ∀ w' (fw : w' < w),
+              arr_rel
+                (ind w' fw τ₁)
+                (termrel' w' (laterlatervr w' fw) τ₂)
+                ts tu
+      in
+      match τ with
+        | ptunit => vrunit ts tu
+        | ptbool => vrbool ts tu
+        | ptprod τ₁ τ₂ => vrprod τ₁ τ₂ ts tu
+        | ptsum τ₁ τ₂ => vrsum τ₁ τ₂ ts tu
+        | ptarr τ₁ τ₂ => vrarr τ₁ τ₂ ts tu
+        | pEmulDV n p => match n with
+                           | 0 => ts = S.unit ∧ p = imprecise
+                           | S n' => (ts = unkUVal (S n') ∧ p = imprecise) ∨
+                                     exists ts',
+                                       (ts = inUnit n' ts' ∧ vrunit ts' tu) ∨
+                                       (ts = inBool n' ts' ∧ vrbool ts' tu) ∨
+                                       (ts = inProd n' ts' ∧ vrprod (pEmulDV n' p) (pEmulDV n' p) ts' tu ∧
+                                        OfTypeUtlc (ptprod (pEmulDV n' p) (pEmulDV n' p)) tu) ∨
+                                       (ts = inSum n' ts' ∧ vrsum (pEmulDV n' p) (pEmulDV n' p) ts' tu ∧ 
+                                        OfTypeUtlc (ptsum (pEmulDV n' p) (pEmulDV n' p)) tu) ∨
+                                       (ts = inArr n' ts' ∧ vrarr (pEmulDV n' p) (pEmulDV n' p) ts' tu ∧ 
+                                        OfTypeUtlc (ptarr (pEmulDV n' p) (pEmulDV n' p)) tu)
+                         end
+      end.
+
+  Definition valrel (w : World) (τ : PTy)(t₁ : S.Tm) (t₂ : U.UTm) : Prop :=
+    Fix lt_wf (fun w => PTRel) valrel' w τ t₁ t₂.
+
+  Lemma valrel_def_funext w (ind₁ ind₂ : ∀ w', w' < w → PTRel) :
+    (∀ w' (fw : w' < w), ind₁ w' fw = ind₂ w' fw) →
+    valrel' w ind₁ = valrel' w ind₂.
+  Proof.
+    intros.
+    enough (ind₁ = ind₂) as -> by auto.
+    extensionality w'.
+    extensionality fw.
+    trivial.
+  Qed.
+
+  Lemma valrel_fixp : ∀ w, valrel w = valrel' w (fun w _ => valrel w).
+  Proof.
+    refine (Fix_eq lt_wf (fun w => PTRel) valrel' valrel_def_funext).
+  Qed.
+
+  Definition contrel (w : World) : PCRel :=
+    contrel' w (fun w fw => valrel w).
+
+  Definition termrel (w : World) : PTRel :=
+    termrel' w (fun w fw => valrel w).
+
+  Lemma termrel_fixp :
+    ∀ w, termrel w = termrel' w (fun w _ => valrel' w (fun w _ => valrel w)).
+  Proof.
+    unfold termrel.
+    intros w.
+    f_equal.
+    (* Should we avoid functional extensionality? *)
+    extensionality w'.
+    extensionality fw.
+    apply valrel_fixp.
+  Qed.
+
+  Definition envrel (w : World) (Γ : PEnv) (γs : Sub S.Tm) (γu : Sub U.UTm) : Prop :=
+    ∀ i τ, ⟪ i : τ p∈ Γ ⟫ → valrel w τ (γs i) (γu i).
+
+  Definition OpenLRN (n : nat) (Γ : PEnv) (ts : S.Tm) (tu : U.UTm) (τ : PTy) : Prop :=
+    ⟪ repEmulCtx Γ ⊢ ts : repEmul τ ⟫ ∧
+    ⟨ pdom Γ ⊢ tu ⟩ ∧
+    ∀ w, lev w ≤ n → ∀ γs γu, envrel w Γ γs γu → termrel w τ (ts [ γs ]) (tu [ γu ]).
+
+  Definition OpenLR (Γ : PEnv) (ts : S.Tm) (tu : U.UTm) (τ : PTy) : Prop :=
+    ∀ n, OpenLRN n Γ ts tu τ.
+
+  Definition OpenLRCtxN (n : nat) (Cs : S.PCtx) (Cu : U.PCtx) (Γ' : PEnv) (τ' : PTy) (Γ : PEnv) (τ : PTy) : Prop :=
+    ⟪ ⊢ Cs : repEmulCtx Γ' , repEmul τ' → repEmulCtx Γ , repEmul τ ⟫ ∧
+    ∀ ts tu, OpenLRN n Γ' ts tu τ' -> OpenLRN n Γ (S.pctx_app ts Cs) (U.pctx_app tu Cu) τ.
+
+  Definition OpenLRCtx (Cs : S.PCtx) (Cu : U.PCtx) (Γ' : PEnv) (τ' : PTy) (Γ : PEnv) (τ : PTy) : Prop :=
+    ⟪ ⊢ Cs : repEmulCtx Γ' , repEmul τ' → repEmulCtx Γ' , repEmul τ ⟫ ∧
+    ∀ ts tu, OpenLR Γ' ts tu τ' → OpenLR Γ (S.pctx_app ts Cs) (U.pctx_app tu Cu) τ.
+
+End LogicalRelation.
+
+Arguments termrel d w τ t₁ t₂ : simpl never.
+Arguments valrel d w τ t₁ t₂ : simpl never.
+Arguments valrel' d w ind !τ !t₁ !t₂ /.
+
+Notation "⟪ Γ ⊩ ts ⟦ d , n ⟧ tu : τ ⟫" := (OpenLRN d n Γ ts tu τ)
+  (at level 0, ts at level 98,
+   d at level 98, n at level 98,
+   tu at level 98,
+   Γ at level 98, τ at level 98,
+   format "⟪ Γ ⊩  ts ⟦ d , n ⟧ tu  :  τ  ⟫").
+
+Notation "⟪ Γ ⊩ ts ⟦ d ⟧ tu : τ ⟫" := (OpenLR d Γ ts tu τ)
+  (at level 0, ts at level 98,
+   d at level 98, tu at level 98,
+   Γ at level 98, τ at level 98,
+   format "⟪ Γ ⊩  ts ⟦ d ⟧ tu  :  τ  ⟫").
+
+Notation "⟪ ⊩ Cs ⟦ d , n ⟧ Cu : Γ₀ , τ₀ → Γ , τ ⟫" := (OpenLRCtxN d n Cs Cu Γ₀ τ₀ Γ τ)
+  (at level 0, Cs at level 98,
+   d at level 98, n at level 98,
+   Cu at level 98,
+   Γ₀ at level 98, τ₀ at level 98,
+   Γ at level 98, τ at level 98,
+   format "⟪  ⊩  Cs ⟦ d , n ⟧ Cu  :  Γ₀ ,  τ₀  →  Γ ,  τ  ⟫").
+
+Notation "⟪ ⊩ Cs ⟦ d ⟧ Cu : Γ₀ , τ₀ → Γ , τ ⟫" := (OpenLRCtx d Cs Cu Γ₀ τ₀ Γ τ)
+  (at level 0, Cs at level 98,
+   d at level 98, Cu at level 98,
+   Γ₀ at level 98, τ₀ at level 98,
+   Γ at level 98, τ at level 98,
+   format "⟪  ⊩  Cs ⟦ d ⟧ Cu  :  Γ₀ ,  τ₀  →  Γ ,  τ  ⟫").
+
+Section TermRelZero.
+  Definition termreli₀ d dfc w τ ts tu :=
+    (∃ vs vu, clos_refl_trans_1n S.Tm S.eval ts vs ∧ U.ctxevalStar tu vu ∧
+              valrel d w τ vs vu) ∨
+    (forall Cs Cu, S.ECtx Cs → U.ECtx Cu → Obs d (lateri dfc w) (S.pctx_app ts Cs) (U.pctx_app tu Cu)).
+
+  Arguments termreli₀ d dfc w τ ts tu : simpl never.
+
+  Definition termrel₀ d w τ ts tu :=
+    termreli₀ d 0 w τ ts tu.
+  
+  Arguments termrel₀ d w τ ts tu : simpl never.
+
+End TermRelZero.
