FixIsMu/LogRelFI/LemmasPseudoType.v
@@ -1,0 +1,222 @@
+Require Import StlcFix.CanForm.
+Require Import StlcFix.LemmasTyping.
+(* Require Import StlcIso.LemmasScoping. *)
+Require Export LogRelFI.PseudoTypeFI.
+Require Import UValFI.UVal.
+
+Section RepEmul.
+  Lemma repEmul_embed_leftinv τ :
+    repEmul (embed τ) = τ.
+  Proof.
+    induction τ; simpl; try f_equal; intuition.
+  Qed.
+
+  Lemma repEmulCtx_embedCtx_leftinv Γ :
+    repEmulCtx (embedCtx Γ) = Γ.
+  Proof.
+    induction Γ; simpl; try f_equal; eauto using repEmul_embed_leftinv.
+  Qed.
+
+End RepEmul.
+
+Ltac crushRepEmulEmbed :=
+  match goal with
+      [ |- context[ repEmul( embed ?τ) ] ] => rewrite -> (repEmul_embed_leftinv τ)
+    | [ |- context[ repEmulCtx( embedCtx ?Γ) ] ] => rewrite -> (repEmulCtx_embedCtx_leftinv Γ)
+  end.
+
+Lemma getevar_repEmulCtx {i τ Γ} :
+  ⟪ i : τ ∈ repEmulCtx Γ ⟫ →
+  exists τ', ⟪ i : τ' p∈ Γ ⟫ ∧ τ = repEmul τ'.
+Proof.
+  revert i. induction Γ as [|Γ IHΓ τ'']; 
+  inversion 1; [idtac| destruct (IHΓ _ H4) as [? [? ?]]];
+  eauto using GetEvarP.
+Qed.
+
+Section OfType.
+
+  Local Ltac crush :=
+    unfold OfType, OfTypeStlcFix, OfTypeStlcIso; intros;
+    repeat
+      (subst;
+       stlcCanForm;
+       crushTyping;
+       I.crushTyping;
+       F.crushTyping;
+       (* crushUtlcScoping; *)
+       destruct_conjs;
+       repeat
+         match goal with
+           | H: False |- _ => elim H
+           | H: True  |- _ => clear H
+           | H: _ ∧ _ |- _ => destruct  H
+           | H: match ?tu with _ => _ end |- _ =>
+             destruct tu eqn: ?; cbn in H
+           | H: _ ∨ _ |- _ => destruct  H
+           | [ |- _ ∧ _ ] => split
+         end); eauto 20.
+
+  Lemma OfType_unit : OfType ptunit F.unit I.unit.
+  Proof. crush. Qed.
+
+  (* Lemma OfType_true : OfType ptbool F.true I.true. *)
+  (* Proof. crush. Qed. *)
+
+  (* Lemma OfType_false : OfType ptbool S.false U.false. *)
+  (* Proof. crush. Qed. *)
+
+  Lemma OfType_inl {τ₁ τ₂ ts tu} :
+    OfType τ₁ ts tu →
+    OfType (ptsum τ₁ τ₂) (F.inl ts) (I.inl tu).
+  Proof. crush. Qed.
+
+  Lemma OfType_inr {τ₁ τ₂ ts tu} :
+    OfType τ₂ ts tu →
+    OfType (ptsum τ₁ τ₂) (F.inr ts) (I.inr tu).
+  Proof. crush. Qed.
+
+  (* Lemma OfType_pair {τ₁ τ₂ ts₁ ts₂ tu₁ tu₂} : *)
+  (*   OfType τ₁ ts₁ tu₁ → *)
+  (*   OfType τ₂ ts₂ tu₂ → *)
+  (*   OfType (ptprod τ₁ τ₂) (S.pair ts₁ ts₂) (U.pair tu₁ tu₂). *)
+  (* Proof. crush. Qed. *)
+
+  Lemma OfType_lambda {τ₁ τ₂ τ₁' tsb tub} :
+    τ₁' = repEmul τ₁ →
+    I.Typing I.empty (I.abs (fxToIs τ₁) tub) (I.tarr (fxToIs τ₁) (fxToIs τ₂)) →
+    ⟪ empty ⊢ F.abs (repEmul τ₁) tsb : repEmul τ₁ ⇒ repEmul τ₂ ⟫ →
+    OfType (ptarr τ₁ τ₂) (F.abs τ₁' tsb) (I.abs (fxToIs τ₁) tub).
+  Proof. crush. Qed.
+
+  Lemma OfType_inversion_ptunit {ts tu} :
+    OfType ptunit ts tu →
+    ts = F.unit ∧ tu = I.unit.
+  Proof.
+    intros.
+    inversion H.
+    unfold OfTypeStlcFix in H0.
+    inversion H1.
+    crush.
+    inversion H0.
+    inversion H.
+  Qed.
+
+  Lemma OfType_inversion_ptbool {ts tu} :
+    OfType ptbool ts tu →
+    ts = S.true ∧ tu = U.true ∨
+    ts = S.true ∧ tu = U.false ∨
+    ts = S.false ∧ tu = U.true ∨
+    ts = S.false ∧ tu = U.false.
+  Proof. crush. Qed.
+
+  Lemma OfType_inversion_ptsum {τ₁ τ₂ ts tu} :
+    OfType (ptsum τ₁ τ₂) ts tu →
+    ∃ ts' tu',
+      ts = S.inl ts' ∧ tu = U.inl tu' ∧ OfType τ₁ ts' tu' ∨
+      ts = S.inl ts' ∧ tu = U.inr tu' ∨
+      ts = S.inr ts' ∧ tu = U.inl tu' ∨
+      ts = S.inr ts' ∧ tu = U.inr tu' ∧ OfType τ₂ ts' tu'.
+  Proof. crush. Qed.
+
+  Lemma OfType_inversion_ptprod {τ₁ τ₂ ts tu} :
+    OfType (ptprod τ₁ τ₂) ts tu →
+    ∃ ts₁ tu₁ ts₂ tu₂,
+      ts = S.pair ts₁ ts₂ ∧
+      tu = U.pair tu₁ tu₂ ∧
+      OfType τ₁ ts₁ tu₁ ∧
+      OfType τ₂ ts₂ tu₂.
+  Proof. crush. Qed.
+
+  Lemma OfTypeUtlc_inversion_ptarr {τ₁ τ₂ tu} :
+    OfTypeUtlc (ptarr τ₁ τ₂) tu →
+    ∃ tu', tu = U.abs tu' ∧ ⟨ 1 ⊢ tu' ⟩.
+  Proof. crush. Qed.
+
+  Lemma OfTypeUtlc_inversion_ptprod {τ₁ τ₂ tu} :
+    OfTypeUtlc (ptprod τ₁ τ₂) tu →
+    ∃ tu₁ tu₂, tu = U.pair tu₁ tu₂ ∧ OfTypeUtlc τ₁ tu₁ ∧ OfTypeUtlc τ₂ tu₂.
+  Proof. crush. Qed.
+
+  Lemma OfTypeUtlc_inversion_ptsum {τ₁ τ₂ tu} :
+    OfTypeUtlc (ptsum τ₁ τ₂) tu →
+    ∃ tu', (tu = U.inl tu' ∧ OfTypeUtlc τ₁ tu') ∨
+           (tu = U.inr tu' ∧ OfTypeUtlc τ₂ tu').
+  Proof. crush. Qed.
+
+  Lemma OfType_inversion_ptarr {τ₁ τ₂ ts tu} :
+    OfType (ptarr τ₁ τ₂) ts tu →
+    ∃ ts' tu',
+      ts = S.abs (repEmul τ₁) ts' ∧
+      tu = U.abs tu' ∧
+      ⟪ empty ▻ repEmul τ₁ ⊢ ts' : repEmul τ₂ ⟫ ∧
+      ⟨ 1 ⊢ tu' ⟩.
+  Proof. crush. Qed.
+
+  Lemma OfType_inversion_pEmulDV {n p ts tu} :
+    OfType (pEmulDV n p) ts tu →
+    S.Value ts ∧ U.Value tu ∧
+    ⟪ empty ⊢ ts : UVal n ⟫ ∧
+    ⟨ 0 ⊢ tu ⟩.
+  Proof. crush. Qed.
+
+  Lemma OfTypeUtlc'_implies_Value {τ tu} :
+    OfTypeUtlc' τ tu →
+    U.Value tu.
+  Proof.
+    revert tu.
+    induction τ; crush.
+  Qed.
+
+  Lemma OfTypeUtlc_implies_Value {τ tu} :
+    OfTypeUtlc τ tu →
+    U.Value tu.
+  Proof.
+    destruct 1 as (ctu & otu).
+    eauto using OfTypeUtlc'_implies_Value.
+  Qed.
+
+  Lemma OfType_implies_Value {τ ts tu} :
+    OfType τ ts tu →
+    S.Value ts ∧ U.Value tu.
+  Proof.
+    unfold OfType, OfTypeStlc.
+    intros ot; destruct_conjs;
+    eauto using OfTypeUtlc_implies_Value.
+  Qed.
+
+  Lemma OfType_pEmulDV {n p ts tu} :
+    S.Value ts ∧ U.Value tu ∧
+    ⟪ empty ⊢ ts : UVal n ⟫ → 
+    ⟨ 0 ⊢ tu ⟩ →
+    OfType (pEmulDV n p) ts tu.
+  Proof. crush. Qed.
+
+End OfType.
+
+Ltac crushOfType :=
+  repeat
+    match goal with
+      | [ H: OfType ptunit _ _ |- _ ] => apply OfType_inversion_ptunit in H
+      | [ H: OfType ptbool _ _ |- _ ] => apply OfType_inversion_ptbool in H
+      | [ H: OfType (ptsum _ _) _ _ |- _ ] => apply OfType_inversion_ptsum in H
+      | [ H: OfType (ptprod _ _) _ _ |- _ ] => apply OfType_inversion_ptprod in H
+      | [ H: OfType (ptarr _ _) _ _ |- _ ] => apply OfType_inversion_ptarr in H
+      | [ H: OfTypeUtlc _ ?t |- ⟨ 0 ⊢ ?t ⟩ ] => exact (proj1 H)
+      | [ H: OfTypeUtlc ?τ ?t |- OfTypeUtlc' ?τ ?t ] => exact (proj2 H)
+      | [ H: OfTypeUtlc (ptarr _ _) _ |- _ ] => apply OfTypeUtlc_inversion_ptarr in H
+      | [ H: OfTypeUtlc (ptprod _ _) _ |- _ ] => apply OfTypeUtlc_inversion_ptprod in H
+      | [ H: OfTypeUtlc (ptsum _ _) _ |- _ ] => apply OfTypeUtlc_inversion_ptsum in H
+      | [ H: OfType (pEmulDV _ _) _ _ |- _ ] => apply OfType_inversion_pEmulDV in H
+      (* | [ H: OfTypeUtlc ptbool ?t  |- _ ] =>  change (OfTypeUtlc ptbool t) with (t = U.true ∨ t = U.false) in H *)
+      (* | [ H: OfTypeUtlc ptunit ?t  |- _ ] => change (OfTypeUtlc ptunit t) with (t = U.unit) in H; subst t *)
+      | [ |- OfType ptunit S.unit U.unit ] => apply OfType_unit
+      | [ |- OfType ptbool S.true U.true ] => apply OfType_true
+      | [ |- OfType ptbool S.false U.false ] => apply OfType_false
+      | [ |- OfType (ptsum _ _) (S.inl _) (U.inl _)] => apply OfType_inl
+      | [ |- OfType (ptsum _ _) (S.inr _) (U.inr _)] => apply OfType_inr
+      | [ |- OfType (ptprod _ _) (S.pair _ _) (U.pair _ _) ] => apply OfType_pair
+      | [ |- OfType (ptarr _ _) (S.abs _ _) (U.abs _) ] => apply OfType_lambda
+      | [ |- OfTypeUtlc _ _ ] => split
+      | [ |- OfType (pEmulDV _ _) _ _ ] => apply OfType_pEmulDV
+    end.
